Backporting typeclasses and record syntax changes, refactoring of classes and records declarations and some bug fixes.
Merged revisions 11563,11572,11587,11655-11658,11660,11679-11681,11684-11686 via svnmerge from 
svn+ssh://msozeau@scm.gforge.inria.fr/svn/coq/trunk

........
  r11563 | msozeau | 2008-11-09 17:17:14 +0100 (Sun, 09 Nov 2008) | 8 lines
  
  More factorization of inductive/record and typeclasses: move class
  declaration code to toplevel/record, including support for singleton
  classes as definitions. Parsing code also factorized. Arnaud: one more
  thing to think about when refactoring the definitions in vernacentries.
  Add support for specifying what to do with anonymous variables in
  contexts during internalisation (fixes bug #1982), current choice is to
  generate a name for typeclass bindings.
........
  r11572 | msozeau | 2008-11-10 12:15:41 +0100 (Mon, 10 Nov 2008) | 3 lines
  
  Fix mixup between Record, Structure and Class by adding a new variant for
  the three cases.
........
  r11587 | msozeau | 2008-11-14 16:29:22 +0100 (Fri, 14 Nov 2008) | 2 lines
  
  Add missing test-suite files for closed bugs.
........
  r11655 | msozeau | 2008-12-04 19:38:23 +0100 (Thu, 04 Dec 2008) | 2 lines
  
  Fixes for unification and substitution of metas under binders.
........
  r11656 | msozeau | 2008-12-04 19:39:28 +0100 (Thu, 04 Dec 2008) | 3 lines
  
  Fix priority of the Leibniz Setoid instance to 10 (thanks to M. Lasson
  for the report).
........
  r11657 | msozeau | 2008-12-04 19:41:10 +0100 (Thu, 04 Dec 2008) | 2 lines
  
  Correct handling of defined methods (let-ins) in instance declarations.
........
  r11658 | msozeau | 2008-12-04 19:42:26 +0100 (Thu, 04 Dec 2008) | 2 lines
  
  Do not catch _all_ exceptions in setoid unification.
........
  r11660 | msozeau | 2008-12-08 06:34:31 +0100 (Mon, 08 Dec 2008) | 3 lines
  
  Fix handling of [inverse] in setoid_rewrite, with an hopefully complete
  procedure. Brainstormed with Nicolas Tabareau.
........
  r11679 | msozeau | 2008-12-14 17:34:43 +0100 (Sun, 14 Dec 2008) | 13 lines
  
  Generalized binding syntax overhaul: only two new binders: `() and `{},
  guessing the binding name by default and making all generalized
  variables implicit. At the same time, continue refactoring of
  Record/Class/Inductive etc.., getting rid of [VernacRecord]
  definitively. The AST is not completely satisfying, but leaning towards 
  Record/Class as restrictions of inductive (Arnaud, anyone ?).
  Now, [Class] declaration bodies are either of the form [meth : type] or 
  [{ meth : type ; ... }], distinguishing singleton "definitional" classes
  and inductive classes based on records. The constructor syntax is
  accepted ([meth1 : type1 | meth1 : type2]) but raises an error
  immediately, as support for defining a class by a general inductive type
  is not there yet (this is a bugfix!).
........
  r11680 | msozeau | 2008-12-14 18:19:47 +0100 (Sun, 14 Dec 2008) | 8 lines
  
  Fixes in the type classes documentation:
  - Document the new binders, now in sync with the implementation
  - Fix the examples
  - Redo the part about superclasses now that we got rid of "=>"
  - Add explanation of singleton "definitional" classes
  - Add info about the optional priority attribute of instances (thanks to
  M. Lasson for pointing it out).
........
  r11681 | msozeau | 2008-12-14 18:23:04 +0100 (Sun, 14 Dec 2008) | 4 lines
  
  Fix looping class resolution bug discovered by B. Aydemir and use the
  right unification flags for exact hints in eauto (may break a lot of 
  things by succeeding much more often).
........
  r11684 | msozeau | 2008-12-16 11:04:16 +0100 (Tue, 16 Dec 2008) | 2 lines
  
  Fix for syntax changes in test-suite scripts.
........
  r11685 | msozeau | 2008-12-16 11:19:06 +0100 (Tue, 16 Dec 2008) | 6 lines
  
  Finish fix for the treatment of [inverse] in [setoid_rewrite], making a
  variant of the [unify] tactic that takes a hint db as argument and does
  unification modulo its [transparent_state]. Add test-file for bug #1939
  and another [AdvancedTypeClasses.v] that mimicks
  [AdvancedCanonicalStructure.v].
........
  r11686 | msozeau | 2008-12-16 13:57:26 +0100 (Tue, 16 Dec 2008) | 6 lines
  
  Move FunctionalExtensionality to Logic/ (someone please check that the
  doc is ok). Rework the .v files in Program accordingly, adding some
  documentation and proper headers. Integrate the development of an
  elimination principle for measured functions in Program/Wf by Eelis van
  der Weegen.
........


git-svn-id: svn+ssh://scm.gforge.inria.fr/svn/coq/branches/v8.2@11709 85f007b7-540e-0410-9357-904b9bb8a0f7

contrib/funind/rawterm_to_relation.ml
@@ -1192,7 +1192,7 @@ let do_build_inductive
   let rel_ind i ext_rel_constructors = 
     ((dummy_loc,relnames.(i)),
     rel_params,
-    rel_arities.(i),
+    Some rel_arities.(i),
     ext_rel_constructors),None
   in
   let ext_rel_constructors = (Array.mapi rel_ind ext_rels_constructors) in 
@@ -1225,7 +1225,7 @@ let do_build_inductive
 	let _time3 = System.get_time () in
 (* 	Pp.msgnl (str "error : "++ str (string_of_float (System.time_difference time2 time3))); *)
 	let repacked_rel_inds = 
-	  List.map  (fun ((a , b , c , l),ntn) -> (a , b, c , Vernacexpr.Constructors l),ntn )
+	  List.map  (fun ((a , b , c , l),ntn) -> ((false,a) , b, c , None, Vernacexpr.Constructors l),ntn )
 	                  rel_inds
 	in
 	let msg = 		     
@@ -1240,7 +1240,7 @@ let do_build_inductive
 	let _time3 = System.get_time () in
 (* 	Pp.msgnl (str "error : "++ str (string_of_float (System.time_difference time2 time3))); *)
 	let repacked_rel_inds = 
-	  List.map  (fun ((a , b , c , l),ntn) -> (a , b, c , Vernacexpr.Constructors l),ntn )
+	  List.map  (fun ((a , b , c , l),ntn) -> ((false,a) , b, c , None, Vernacexpr.Constructors l),ntn )
 	                  rel_inds
 	in
 	let msg = 		     
