contrib/interface/xlate.ml
@@ -1969,24 +1969,24 @@ let rec xlate_vernac =
 	       translated_restriction)
   	| SearchAbout [] -> assert false)
 
-  | (*Record from tactics/Record.v *)
-    VernacRecord 
-      (_, (add_coercion, (_,s)), binders, c1,
-       rec_constructor_or_none, field_list) ->
-      let record_constructor =
-        xlate_ident_opt (Option.map snd rec_constructor_or_none) in
-      CT_record
-       ((if add_coercion then CT_coercion_atm else
-          CT_coerce_NONE_to_COERCION_OPT(CT_none)),
-        xlate_ident s, xlate_binder_list binders, 
-	xlate_formula c1, record_constructor,
-         build_record_field_list field_list)
+(*   | (\*Record from tactics/Record.v *\) *)
+(*     VernacRecord  *)
+(*       (_, (add_coercion, (_,s)), binders, c1, *)
+(*        rec_constructor_or_none, field_list) -> *)
+(*       let record_constructor = *)
+(*         xlate_ident_opt (Option.map snd rec_constructor_or_none) in *)
+(*       CT_record *)
+(*        ((if add_coercion then CT_coercion_atm else *)
+(*           CT_coerce_NONE_to_COERCION_OPT(CT_none)), *)
+(*         xlate_ident s, xlate_binder_list binders,  *)
+(* 	xlate_formula (Option.get c1), record_constructor, *)
+(*          build_record_field_list field_list) *)
    | VernacInductive (isind, lmi) ->
       let co_or_ind = if isind then "Inductive" else "CoInductive" in
-      let strip_mutind = function 
-	  (((_,s), parameters, c, Constructors constructors), notopt) ->
+      let strip_mutind = function
+          (((_, (_,s)), parameters, c, _, Constructors constructors), notopt) ->
           CT_ind_spec
-            (xlate_ident s, xlate_binder_list parameters, xlate_formula c,
+            (xlate_ident s, xlate_binder_list parameters, xlate_formula (Option.get c),
              build_constructors constructors,
 	     translate_opt_notation_decl notopt) 
 	| _ -> xlate_error "TODO: Record notation in (Co)Inductive" in
@@ -2148,7 +2148,7 @@ let rec xlate_vernac =
 
     (* Type Classes *) 
    | VernacDeclareInstance _|VernacContext _|
-	 VernacInstance (_, _, _, _, _)|VernacClass (_, _, _, _, _) ->
+	 VernacInstance (_, _, _, _, _) ->
 	   xlate_error "TODO: Type Classes commands"
 
   | VernacResetName id -> CT_reset (xlate_ident (snd id))
