parsing/pcoq.mli
@@ -167,6 +167,7 @@ module Constr :
     val binders_let : local_binder list Gram.Entry.e
     val binders_let_fixannot : (local_binder list * (identifier located option * recursion_order_expr)) Gram.Entry.e
     val typeclass_constraint : (name located * bool * constr_expr) Gram.Entry.e
+    val record_declaration : constr_expr Gram.Entry.e
     val appl_arg : (constr_expr * explicitation located option) Gram.Entry.e
   end
 
