proofs/clenvtac.mli
@@ -21,8 +21,8 @@ open Unification
 (*i*)
 
 (* Tactics *)
-val unify : constr -> tactic
-val clenv_refine : evars_flag -> clausenv -> tactic
+val unify : ?flags:unify_flags -> constr -> tactic
+val clenv_refine : evars_flag -> ?with_classes:bool -> clausenv -> tactic
 val res_pf : clausenv -> ?with_evars:evars_flag -> ?allow_K:bool -> ?flags:unify_flags -> tactic
 val elim_res_pf_THEN_i : clausenv -> (clausenv -> tactic array) -> tactic
 
