toplevel/record.mli
@@ -15,6 +15,7 @@ open Sign
 open Vernacexpr
 open Topconstr
 open Impargs
+open Libnames
 (*i*)
 
 (* [declare_projections ref name coers params fields] declare projections of
@@ -27,15 +28,13 @@ val declare_projections :
   (name * bool) list * constant option list
 
 val declare_structure : bool (*coinductive?*)-> identifier -> identifier -> 
-  manual_explicitation list -> rel_context -> (* params *)
-  Term.constr -> (* arity *)
+  manual_explicitation list -> rel_context -> (* params *) constr -> (* arity *)
   Impargs.manual_explicitation list list -> Sign.rel_context -> (* fields *)
   ?kind:Decl_kinds.definition_object_kind -> ?name:identifier ->
   bool -> (* coercion? *)
   bool list -> (* field coercions *)
-  mutual_inductive
+  inductive
 
 val definition_structure :
-  bool (*coinductive?*)*lident with_coercion * local_binder list *
-  (local_decl_expr with_coercion with_notation) list * 
-  identifier * constr_expr -> kernel_name
+  record_kind * bool (*coinductive?*)*lident with_coercion * local_binder list *
+  (local_decl_expr with_coercion with_notation) list * identifier * sorts option -> global_reference
