toplevel/vernacentries.ml
@@ -372,23 +372,31 @@ let vernac_assumption kind l nl=
 	  else Dumpglob.dump_definition lid true "var") idl;
       declare_assumption idl is_coe kind [] c false false nl) l
 
-let vernac_record finite struc binders sort nameopt cfs =
+let vernac_record k finite struc binders sort nameopt cfs =
   let const = match nameopt with 
     | None -> add_prefix "Build_" (snd (snd struc))
     | Some (_,id as lid) ->
-	if Dumpglob.dump () then Dumpglob.dump_definition lid false "constr"; id in
+	Dumpglob.dump_definition lid false "constr"; id in
+  let sigma = Evd.empty in
+  let env = Global.env() in
+  let s = Option.map (fun x ->
+    let s = Reductionops.whd_betadeltaiota env sigma (interp_constr sigma env x) in
+      match kind_of_term s with
+      | Sort s -> s
+      | _ -> user_err_loc
+          (constr_loc x,"definition_structure", str "Sort expected.")) sort
+  in
     if Dumpglob.dump () then (
-	Dumpglob.dump_definition (snd struc) false "rec";
-	List.iter (fun ((_, x), _) ->
-	  match x with
-	    | AssumExpr ((loc, Name id), _) -> Dumpglob.dump_definition (loc,id) false "proj"
-	    | _ -> ()) cfs);
-    ignore(Record.definition_structure (finite,struc,binders,cfs,const,sort))
-
-
+      Dumpglob.dump_definition (snd struc) false "rec";
+      List.iter (fun ((_, x), _) ->
+	match x with
+	| Vernacexpr.AssumExpr ((loc, Name id), _) -> Dumpglob.dump_definition (loc,id) false "proj"
+	| _ -> ()) cfs);
+    ignore(Record.definition_structure (k,finite,struc,binders,cfs,const,s))
+      
 let vernac_inductive finite indl = 
   if Dumpglob.dump () then
-    List.iter (fun ((lid, _, _, cstrs), _) ->
+    List.iter (fun (((coe,lid), _, _, _, cstrs), _) ->
       match cstrs with 
       | Constructors cstrs ->
 	  Dumpglob.dump_definition lid false"ind";
@@ -397,15 +405,25 @@ let vernac_inductive finite indl =
       | _ -> () (* dumping is done by vernac_record (called below) *) )
     indl;
   match indl with
-    | [ ( id , bl , c ,RecordDecl (oc,fs) ), None ] -> 
-        vernac_record finite (false,id) bl c oc fs
-    | [ ( _ , _ , _ , RecordDecl _ ) , _ ] -> 
-        Util.error "where clause not supported for (co)inductive records"
-    | _ -> let unpack = function 
-        | ( id , bl , c , Constructors l ) , ntn  -> ( id , bl , c , l ) , ntn
- 	| _ -> Util.error "Cannot handle mutually (co)inductive records."
-      in
-      let indl = List.map unpack indl in
+  | [ ( id , bl , c , Some b, RecordDecl (oc,fs) ), None ] -> 
+      vernac_record (match b with Class true -> Class false | _ -> b)
+	finite id bl c oc fs
+  | [ ( id , bl , c , Some (Class true), Constructors [l]), _ ] -> 
+      let f = 
+	let (coe, ((loc, id), ce)) = l in
+	  ((coe, AssumExpr ((loc, Name id), ce)), None)
+      in vernac_record (Class true) finite id bl c None [f]
+  | [ ( id , bl , c , Some (Class true), _), _ ] -> 
+      Util.error "Definitional classes must have a single method"
+  | [ ( id , bl , c , Some (Class false), Constructors _), _ ] ->
+      Util.error "Inductive classes not supported"
+  | [ ( _ , _ , _ , _, RecordDecl _ ) , _ ] -> 
+      Util.error "where clause not supported for (co)inductive records"
+  | _ -> let unpack = function 
+      | ( (_, id) , bl , c , _ , Constructors l ) , ntn  -> ( id , bl , c , l ) , ntn
+      | _ -> Util.error "Cannot handle mutually (co)inductive records."
+    in
+    let indl = List.map unpack indl in
       Command.build_mutual indl finite
 
 let vernac_fixpoint l b = 
@@ -603,11 +621,6 @@ let vernac_identity_coercion stre id qids qidt =
   Class.try_add_new_identity_coercion id stre source target
 
 (* Type classes *)
-let vernac_class id par ar sup props =
-  if Dumpglob.dump () then (
-      Dumpglob.dump_definition id false "class";
-      List.iter (fun (lid, _, _) -> Dumpglob.dump_definition lid false "meth") props);
-  Classes.new_class id par ar sup props
  
 let vernac_instance glob sup inst props pri =
   Dumpglob.dump_constraint inst false "inst";
@@ -1321,7 +1334,6 @@ let interp c = match c with
 
   | VernacEndSegment lid -> vernac_end_segment lid
 
-  | VernacRecord ((_,finite),id,bl,s,idopt,fs) -> vernac_record finite id bl s idopt fs
   | VernacRequire (export,spec,qidl) -> vernac_require export spec qidl
   | VernacImport (export,qidl) -> vernac_import export qidl
   | VernacCanonical qid -> vernac_canonical qid
@@ -1329,8 +1341,6 @@ let interp c = match c with
   | VernacIdentityCoercion (str,(_,id),s,t) -> vernac_identity_coercion str id s t
 
   (* Type classes *)
-  | VernacClass (id, par, ar, sup, props) -> vernac_class id par ar sup props
-
   | VernacInstance (glob, sup, inst, props, pri) -> vernac_instance glob sup inst props pri
   | VernacContext sup -> vernac_context sup
   | VernacDeclareInstance id -> vernac_declare_instance id
