test-suite/success/Generalization.v
@@ -2,7 +2,7 @@
 Check `(a = 0).
 Check `(a = 0)%type.
 Definition relation A := A -> A -> Prop.
-Definition equivalence {(R : relation A)} := True.
+Definition equivalence `(R : relation A) := True.
 Check (`(@equivalence A R)).
 
 Definition a_eq_b : `( a = 0 /\ a = b /\ b > c \/ d = e /\ d = 1).
