test-suite/bugs/closed/shouldsucceed/1900.v
@@ -1,0 +1,8 @@
+Parameter A : Type .
+
+Definition eq_A := @eq A.
+
+Goal forall x, eq_A x x.
+intros.
+reflexivity.
+Qed.
