theories/Program/Program.v
@@ -1,3 +1,12 @@
+(************************************************************************)
+(*  v      *   The Coq Proof Assistant  /  The Coq Development Team     *)
+(* <O___,, * CNRS-Ecole Polytechnique-INRIA Futurs-Universite Paris Sud *)
+(*   \VV/  **************************************************************)
+(*    //   *      This file is distributed under the terms of the       *)
+(*         *       GNU Lesser General Public License Version 2.1        *)
+(************************************************************************)
+(* $Id$ *)
+
 Require Export Coq.Program.Utils.
 Require Export Coq.Program.Wf.
 Require Export Coq.Program.Equality.
