theories/Program/Syntax.v
@@ -1,4 +1,3 @@
-(* -*- coq-prog-args: ("-emacs-U") -*- *)
 (************************************************************************)
 (*  v      *   The Coq Proof Assistant  /  The Coq Development Team     *)
 (* <O___,, * CNRS-Ecole Polytechnique-INRIA Futurs-Universite Paris Sud *)
@@ -6,14 +5,15 @@
 (*    //   *      This file is distributed under the terms of the       *)
 (*         *       GNU Lesser General Public License Version 2.1        *)
 (************************************************************************)
+(* $Id$ *)
 
-(* Custom notations and implicits for Coq prelude definitions.
- *
- * Author: Matthieu Sozeau
- * Institution: LRI, CNRS UMR 8623 - UniversitÃcopyright Paris Sud
- *              91405 Orsay, France *)
+(** Custom notations and implicits for Coq prelude definitions.
 
-(** Notations for the unit type and value. *)
+   Author: Matthieu Sozeau
+   Institution: LRI, CNRS UMR 8623 - UniversitÃcopyright Paris Sud
+   91405 Orsay, France *)
+
+(** Notations for the unit type and value à la Haskell. *)
 
 Notation " () " := Datatypes.unit : type_scope.
 Notation " () " := tt.
@@ -42,7 +42,7 @@ Notation " [ ] " := nil : list_scope.
 Notation " [ x ] " := (cons x nil) : list_scope.
 Notation " [ x ; .. ; y ] " := (cons x .. (cons y nil) ..) : list_scope.
 
-(** n-ary exists *)
+(** Treating n-ary exists *)
 
 Notation " 'exists' x y , p" := (ex (fun x => (ex (fun y => p))))
   (at level 200, x ident, y ident, right associativity) : type_scope.
